msp_mq_intt

glue/generic_falcon_lemmas.dfy
@@ -222,6 +222,125 @@ abstract module generic_falcon_lemmas {
         INTT.build_loop_view(s, d)
     }
 
+    function inverse_lsize(view: INTT.loop_view): (r: pow2_t)
+        requires view.loop_view_wf();
+        ensures r.full <= N.full
+    {
+        view.lsize()
+    }
+
+    predicate inverse_ntt_eval_all(a: seq<nat>, coeffs: seq<nat>)
+    {
+        && valid_elems(a)
+        && valid_elems(coeffs)
+        && INTT.ntt_eval_all(as_elems(a), as_elems(coeffs))
+    }
+
+    predicate inverse_t_loop_inv(a: seq<nat>, d: pow2_t, coeffs: seq<nat>)
+        requires 0 <= d.exp <= N.exp;
+    {
+        && valid_elems(a)
+        && valid_elems(coeffs)
+        && INTT.t_loop_inv(as_elems(a), d, as_elems(coeffs))
+    }
+
+    predicate inverse_s_loop_inv(a: seq<nat>, d: pow2_t, j: nat, bi: nat, view: INTT.loop_view)
+    {
+        && valid_elems(a)
+        && view.s_loop_inv(as_elems(a), d, j, bi)
+    }
+
+    predicate inverse_j_loop_inv(a: seq<nat>, d: pow2_t, j: nat, u: nat, view: INTT.loop_view)
+    {
+        && valid_elems(a)
+        && u == j * (2 * d.full)
+        && view.j_loop_inv(as_elems(a), d, j)
+    }
+
+    lemma inverse_t_loop_inv_pre_lemma(coeffs: seq<nat>)
+        requires valid_elems(coeffs);
+        ensures N.exp <= N.exp; // ??
+        ensures inverse_t_loop_inv(coeffs, N, coeffs);
+    {
+        INTT.t_loop_inv_pre_lemma(as_elems(coeffs));
+    }
+
+    lemma inverse_t_loop_inv_post_lemma(a: seq<nat>, one: pow2_t, coeffs: seq<nat>)
+        requires one.exp == 0 <= N.exp;
+        requires inverse_t_loop_inv(a, one, coeffs);
+        ensures inverse_ntt_eval_all(a, coeffs);
+    {
+        INTT.t_loop_inv_post_lemma(a, one, coeffs);
+    }
+
+    predicate inverse_s_loop_update(
+        a: seq<nat>,
+        a': seq<nat>,
+        d: pow2_t,
+        j: nat,
+        bi: nat,
+        s: nat,
+        e: nat,
+        o: nat,
+        view: INTT.loop_view)
+
+        requires inverse_s_loop_inv(a, d, j, bi, view);
+        requires bi < d.full
+    {
+        && e < Q
+        && o < Q
+        && |a'| == |a|
+        && s + d.full < |a|
+        && a'[s + d.full] == o
+        && a'[s] == e
+        && a' == a[s + d.full := o][s := e]
+        && assert valid_elems(a') by {
+            reveal valid_elems();
+        }
+        && view.s_loop_update(as_elems(a), as_elems(a'), d, j, bi)
+    }
+
+    lemma inverse_s_loop_inv_peri_lemma(a: seq<nat>,
+        a': seq<nat>,
+        d: pow2_t,
+        j: nat,
+        bi: nat,
+        s: nat,
+        e: nat,
+        o: nat,
+        view: INTT.loop_view)
+
+        requires inverse_s_loop_inv(a, d, j, bi, view);
+        requires bi < d.full
+        requires inverse_s_loop_update(a, a', d, j, bi, s, e, o, view);
+        ensures inverse_s_loop_inv(a', d, j, bi+1, view);
+    {
+        view.s_loop_inv_peri_lemma(a, a', d, j, bi);
+        assert valid_elems(a') by {
+            reveal valid_elems();
+        }
+    }
+
+    lemma inverse_j_loop_inv_pre_lemma(a: seq<nat>, d: pow2_t, view: INTT.loop_view)
+        requires 0 <= d.exp < N.exp;
+        requires inverse_t_loop_inv(a, pow2_double(d), view.coefficients);
+        requires view.loop_view_wf();
+        requires view.hsize == CPV.block_size(d);
+        ensures inverse_j_loop_inv(a, d, 0, 0, view);
+    {
+        view.j_loop_inv_pre_lemma(as_elems(a), d);
+    }
+
+    lemma inverse_j_loop_inv_post_lemma(a: seq<nat>, d: pow2_t, j: nat, u: nat, view: INTT.loop_view)
+        requires inverse_j_loop_inv(a, d, j, u, view);
+        requires j == view.lsize().full;
+        requires 0 <= view.hsize.exp <= N.exp;
+        requires view.hsize == CPV.block_size(d);
+        ensures INTT.t_loop_inv(a, d, view.coefficients);
+    {
+        view.j_loop_inv_post_lemma(a, d, j);
+    }
+
 // bit rev wraps
 
     function {:opaque} ftable_cast(ftable: seq<nat>): (r: seq<(nat, nat)>)
