glue/msp430/falcon/mq_arith_lemmas.dfy
@@ -302,33 +302,33 @@ module mq_arith_lemmas refines generic_falcon_lemmas {
         ensures |FNTT.rev_mixed_powers_mont_table()| == N.full;
         ensures FNTT.rev_mixed_powers_mont_table()[t.full + j] == 
             MQP.mqmul(FNTT.rev_mixed_powers_mont_x_value(2 * j, d), R);
-        {
-            view.s_loop_inv_pre_lemma(as_elems(a), d, j);
-            FNTT.rev_mixed_powers_mont_table_lemma(t, d, j);
+    {
+        view.s_loop_inv_pre_lemma(as_elems(a), d, j);
+        FNTT.rev_mixed_powers_mont_table_lemma(t, d, j);
 
-            assert u == j * (2 * d.full);
-            assert d == view.hcount();
+        assert u == j * (2 * d.full);
+        assert d == view.hcount();
 
-            var p := pow2_mul(t, d);
-            assert p.exp == 8;
-            assume p.full == 256;
+        var p := pow2_mul(t, d);
+        assert p.exp == 8;
+        assume p.full == 256;
 
-            calc {
-                u;
-                j * (2 * d.full);
-                <= 
-                {
-                    LemmaMulInequality(j, t.full, 2 * d.full);
-                }
-                t.full * (2 * d.full);
-                {
-                    LemmaMulProperties();
-                }
-                2 * (t.full * d.full);
-                2 * p.full;
-                512;
+        calc {
+            u;
+            j * (2 * d.full);
+            <= 
+            {
+                LemmaMulInequality(j, t.full, 2 * d.full);
             }
+            t.full * (2 * d.full);
+            {
+                LemmaMulProperties();
+            }
+            2 * (t.full * d.full);
+            2 * p.full;
+            512;
         }
+    }
 
     lemma forward_s_loop_inv_post_lemma(
         a: seq<nat>,
@@ -383,6 +383,135 @@ module mq_arith_lemmas refines generic_falcon_lemmas {
         returns (gs: nat)
 
         requires forward_s_loop_inv(a, d, j, bi, view);
+        requires bi < d.full
+        requires 2 * d.full < BASE_16;
+        requires s == (bi + j * (2 * d.full)) * 2;
+
+        ensures s == 2 * gs;
+        ensures s + 2 * d.full == 2 * (gs + d.full);
+        ensures gs + d.full < N.full;
+        ensures a[gs] == CPV.level_points_view(a, view.hsize)[bi][2*j];
+        ensures gs == CPV.point_view_index(bi, 2*j, view.hsize);
+        ensures a[gs+d.full] == CPV.level_points_view(a, view.hsize)[bi][2*j+1];
+        ensures gs+d.full == CPV.point_view_index(bi, 2*j+1, view.hsize);
+        ensures a[gs+d.full] < Q;
+        ensures a[gs] < Q;
+    {
+        gs := view.higher_points_view_index_lemma(as_elems(a), d, j, bi);
+        assert s == 2 * gs by {
+            LemmaMulProperties();
+        }
+        reveal valid_elems();
+    }
+
+    lemma inverse_s_loop_inv_pre_lemma(
+        a: seq<nat>,
+        d: pow2_t,
+        j: uint16,
+        t: pow2_t,
+        u: uint16,
+        w: uint16,
+        s: uint16,
+        s_end: uint16,
+        view: INTT.loop_view)
+
+        requires inverse_j_loop_inv(a, d, j, u, view);
+        requires t == view.lsize();
+        requires j < view.lsize().full;
+        requires var w0 := uint16_add(t.full, j);
+            w == uint16_add(w0, w0);
+        requires s == uint16_add(u, u);
+        requires d.full * 2 < BASE_16;
+        requires s_end == uint16_add(d.full * 2, s);
+        ensures s == 2 * u;
+        ensures s_end == (d.full + u) * 2;
+        ensures w == (t.full + j) * 2;
+        ensures inverse_s_loop_inv(a, d, j, 0, view);
+        ensures t.full + j < N.full;
+        ensures |INTT.rev_omega_inv_powers_mont_table()| == N.full;
+        ensures INTT.rev_omega_inv_powers_mont_table()[t.full + j] == 
+            MQP.mqmul(INTT.rev_omega_inv_powers_x_value(2 * j, d), R);
+    {
+        view.s_loop_inv_pre_lemma(as_elems(a), d, j);
+        INTT.rev_omega_inv_powers_mont_table_lemma(t, d, j);
+
+        assert u == j * (2 * d.full);
+        assert d == view.hcount();
+
+        var p := pow2_mul(t, d);
+        assert p.exp == 8;
+        assume p.full == 256;
+
+        calc {
+            u;
+            j * (2 * d.full);
+            <= 
+            {
+                LemmaMulInequality(j, t.full, 2 * d.full);
+            }
+            t.full * (2 * d.full);
+            {
+                LemmaMulProperties();
+            }
+            2 * (t.full * d.full);
+            2 * p.full;
+            512;
+        }
+    }
+
+    lemma inverse_s_loop_inv_post_lemma(
+        a: seq<nat>,
+        d: pow2_t,
+        j: nat,
+        u: uint16,
+        bi: nat,
+        view: INTT.loop_view)
+    
+        requires bi == d.full;
+        requires 2 * d.full < BASE_16;
+        requires u == j * (2 * d.full);
+        requires inverse_s_loop_inv(a, d, j, bi, view);
+
+        ensures uint16_add(2 * d.full, u) == (j + 1) * (2 * d.full);
+        ensures inverse_j_loop_inv(a, d, j + 1, u + 2 * d.full, view);
+    {
+        view.s_loop_inv_post_lemma(as_elems(a), d, j, bi);
+
+        var t := view.lsize();
+        var p := pow2_mul(t, d);
+        assert p.exp == 8;
+        assume p.full == 256;
+
+        assert u + 2 * d.full == (j + 1) * (2 * d.full) by{
+            LemmaMulProperties();
+        }
+
+        calc {
+            (j + 1) * (2 * d.full);
+            <= 
+            {
+                LemmaMulInequality(j+1, t.full, 2 * d.full);
+            }
+            t.full * (2 * d.full);
+            {
+                LemmaMulProperties();
+            }
+            2 * (t.full * d.full);
+            2 * p.full;
+            512;
+        }
+    }
+
+    lemma inverse_s_loop_index_lemma(
+        a: seq<nat>,
+        d: pow2_t,
+        j: nat,
+        s: uint16,
+        bi: nat,
+        view: INTT.loop_view)
+        returns (gs: nat)
+
+        requires inverse_s_loop_inv(a, d, j, bi, view);
         requires bi < d.full
         requires 2 * d.full < BASE_16;
         requires s == (bi + j * (2 * d.full)) * 2;
